CounterDomain.dfy
@@ -47,7 +47,7 @@ module AppCore {
   function Inc(): D.Action { D.Inc }
   function Dec(): D.Action { D.Dec }
 
-  function Dispatch(h: K.History, a: D.Action): K.History { K.Do(h, a) }
+  function Dispatch(h: K.History, a: D.Action): K.History requires K.HistInv(h) { K.Do(h, a) }
   function Undo(h: K.History): K.History { K.Undo(h) }
   function Redo(h: K.History): K.History { K.Redo(h) }
 
